refactor: `HashDict(.Raw)` -> `TDict`

LeanPy/Data/Dict/Basic.lean
@@ -9,7 +9,7 @@ namespace LeanPy
 
 abbrev Hash := UInt64
 
-namespace HashDict
+namespace TDict
 
 inductive Entry (α : Type u) (β : Type v) where
 | protected none
@@ -85,9 +85,6 @@ where go bucket := do
       else go t
     else go t
 
-@[inline] def Internal.isBEqM [Pure m] [BEq α] (k₁ k₂ : α) : m (ULift Bool) :=
-  pure <| .up <| k₁ == k₂
-
 structure Buckets where
   toArray : Array Bucket
   size_toArray_pos : 0 < toArray.size
@@ -137,22 +134,42 @@ def push (hash : Hash) (entryIdx : Nat) (self : Buckets) : Buckets :=
 
 end Buckets
 
-/-- Implementation detail of `HashDict`. -/
-structure Raw (α : Type u) (β : Type v) where
+end TDict
+
+/-- A pure insertion-ordered dictionary of Lean-typed key-value pairs. -/
+structure TDict (α : Type u) (β : Type v) where
   size : Nat
-  buckets : Buckets
-  entries : Array (Entry α β)
+  buckets : TDict.Buckets
+  entries : Array (TDict.Entry α β)
   deriving Nonempty
 
-namespace Raw
+namespace TDict
 
-def emptyWithCapacity (capacity : Nat) : Raw α β where
+def emptyWithCapacity (capacity : Nat) : TDict α β where
   size := 0
   buckets := .emptyWithCapacity capacity
   entries := .emptyWithCapacity capacity
 
+def empty : TDict α β :=
+  emptyWithCapacity 8
+
+instance : EmptyCollection (TDict α β) := ⟨empty⟩
+instance : Nonempty (TDict α β) := ⟨empty⟩
+
+@[inline] def isEmpty (self : TDict α β) : Bool :=
+  self.size == 0
+
+def items (self : TDict α β) : Array (α × β) :=
+  self.entries.filterMap (·.toOption)
+
+def keys (self : TDict α β) : Array α :=
+  self.entries.filterMap (·.key?)
+
+def values (self : TDict α β) : Array β :=
+  self.entries.filterMap (·.value?)
+
 /-- Copies all the entries from `es` into `self` (which should be a new dictionary). -/
-def reinsert (es : Array (Entry α β)) (self : Raw α β)  : Raw α β :=
+def reinsert (es : Array (Entry α β)) (self : TDict α β)  : TDict α β :=
   es.foldl (init := self) fun self e =>
     match e with
     | .none => self
@@ -163,7 +180,7 @@ def reinsert (es : Array (Entry α β)) (self : Raw α β)  : Raw α β :=
       ⟨size, buckets, entries⟩
 
 /-- Remove erased entries from the dictionary. -/
-def compress (self : Raw α β) : Raw α β :=
+def compress (self : TDict α β) : TDict α β :=
   let {size, buckets := _, entries} := self
   reinsert entries {
     size
@@ -172,7 +189,7 @@ def compress (self : Raw α β) : Raw α β :=
   }
 
 /-- Copies all the entries from `self` into a new dictionary with a larger capacity. -/
-def expand {α β} (self : Raw α β) : Raw α β :=
+def expand {α β} (self : TDict α β) : TDict α β :=
   let {size, buckets, entries} := self
   reinsert entries {
     size
@@ -180,20 +197,17 @@ def expand {α β} (self : Raw α β) : Raw α β :=
     entries := .emptyWithCapacity size.nextPowerOfTwo
   }
 
-@[inline] def expandIfNecessary (self : Raw α β) : Raw α β :=
+@[inline] def expandIfNecessary (self : TDict α β) : TDict α β :=
   if Internal.numBucketsForCapacity self.size ≤ self.buckets.size then
     self
   else
     self.expand
 
-def pushCore (hash : Hash) (k : α) (v : β) (self : Raw α β) : Raw α β :=
+def pushCore (hash : Hash) (k : α) (v : β) (self : TDict α β) : TDict α β :=
   let {size, buckets, entries} := self
   let buckets := buckets.push hash entries.size
   let entries := entries.push (.some hash k v)
   expandIfNecessary ⟨size + 1, buckets, entries⟩
-
-@[inline] def push [Hashable α] (k : α) (v : β) (self : Raw α β) : Raw α β :=
-  self.pushCore (hash k) k v
 
 /--
 Looks for the first entry in the bucket identified by `hash`
@@ -201,8 +215,8 @@ whose key satisfies `isBEq`. If none, insert a `k => v` mapping into
 the dictionary. Otherwise, set that entry said mapping.
 -/
 @[specialize] def insertCoreM [Monad m]
-  (hash : Hash) (k : α) (v : β) (self : Raw α β) (isBEq : α → m (ULift Bool))
-: m (Raw α β) := do
+  (hash : Hash) (k : α) (v : β) (self : TDict α β) (isBEq : α → m (ULift Bool))
+: m (TDict α β) := do
   let {size, buckets, entries} := self
   let i := buckets.getIdx hash
   let bucket := buckets.getByIdx i
@@ -215,10 +229,6 @@ the dictionary. Otherwise, set that entry said mapping.
     let entries := entries.push (.some hash k v)
     return expandIfNecessary {size := size + 1, buckets, entries}
 
-@[inline] def insert
-  [Hashable α] [BEq α] (k : α) (v : β) (self : Raw α β)
-: Raw α β := Id.run <| self.insertCoreM (hash k) k v (Internal.isBEqM k)
-
 /--
 Finds the first entry in the bucket identified by `hash`
 whose key satisfies `isBEq` (if any) and erases it from the dictionary.
@@ -227,8 +237,8 @@ This is done by setting the matching entry to `Entry.none`.
 It does not remove the entry index from the bucket.
 -/
 @[specialize] def eraseCoreM [Monad m]
-  (hash : Hash) (self : Raw α β) (isBEq : α → m (ULift Bool))
-: m (Raw α β) := do
+  (hash : Hash) (self : TDict α β) (isBEq : α → m (ULift Bool))
+: m (TDict α β) := do
   let {size, buckets, entries} := self
   let ⟨entryIdx⟩ ← Internal.findEntryIdxM (buckets.get hash) entries isBEq
   if h' : entryIdx < entries.size then
@@ -237,23 +247,39 @@ It does not remove the entry index from the bucket.
   else
     return {size, buckets, entries}
 
+/-! ## Operations for dictionaries with pure keys -/
+
+@[inline] def push [Hashable α] (self : TDict α β)  (k : α) (v : β) : TDict α β :=
+  self.pushCore (hash k) k v
+
+@[inline] def Internal.isBEqM [Pure m] [BEq α] (k₁ k₂ : α) : m (ULift Bool) :=
+  pure <| .up <| k₁ == k₂
+
+@[inline] def insert
+  [Hashable α] [BEq α] (self : TDict α β) (k : α) (v : β)
+: TDict α β := Id.run <| self.insertCoreM (hash k) k v (Internal.isBEqM k)
+
+@[specialize] def ofArray [Hashable α] [BEq α] (items : Array (α × β)) : TDict α β :=
+  items.foldl (init := emptyWithCapacity items.size) fun d (k, v) =>
+    d.insert k v
+
 @[inline] def erase
-  [Hashable α] [BEq α] (k : α) (self : Raw α β)
-: Raw α β := Id.run <| self.eraseCoreM (hash k) (Internal.isBEqM k)
+  [Hashable α] [BEq α] (self : TDict α β) (k : α)
+: TDict α β := Id.run <| self.eraseCoreM (hash k) (Internal.isBEqM k)
 
 @[inline] def getEntryIdxCoreM [Monad m]
-  (hash : Hash) (self : Raw α β) (isBEq : α → m (ULift Bool))
+  (hash : Hash) (self : TDict α β) (isBEq : α → m (ULift Bool))
 : m (ULift Nat) :=
   let {buckets, entries, ..} := self
   Internal.findEntryIdxM (buckets.get hash) entries isBEq
 
 @[inline] def getEntryIdx
-  [Hashable α] [BEq α] (k : α) (self : Raw α β)
+  [Hashable α] [BEq α] (k : α) (self : TDict α β)
 : Nat := ULift.down.{0,0} <| Id.run do
   self.getEntryIdxCoreM (hash k) (Internal.isBEqM k)
 
 @[inline] def contains
-  [Hashable α] [BEq α] (k : α) (self : Raw α β)
+  [Hashable α] [BEq α] (k : α) (self : TDict α β)
 : Bool :=
   let i := self.getEntryIdx k
   if h : i < self.entries.size then
@@ -261,102 +287,52 @@ It does not remove the entry index from the bucket.
   else false
 
 @[inline] def get?
-  [Hashable α] [BEq α] (k : α) (self : Raw α β)
+  [Hashable α] [BEq α] (k : α) (self : TDict α β)
 : Option β :=
   let i := self.getEntryIdx k
   if h : i < self.entries.size then
     self.entries[i].value?
   else none
 
-end Raw
-end HashDict
-
-/-- An insertion-ordered dictionary backed by a `Std.HashMap`. -/
-structure HashDict (α : Type u) (β : Type v) where
-  raw : HashDict.Raw α β
-
-namespace HashDict
-
-def emptyWithCapacity (capacity : Nat) : HashDict α β where
-  raw := .emptyWithCapacity capacity
-
-def empty : HashDict α β :=
-  emptyWithCapacity 8
-
-instance : EmptyCollection (HashDict α β) := ⟨empty⟩
-instance : Nonempty (HashDict α β) := ⟨empty⟩
-
-@[inline] def size (self : HashDict α β) : Nat :=
-  self.raw.size
-
-@[inline] def entries (self : HashDict α β) : Array (Entry α β) :=
-  self.raw.entries
-
-def items (self : HashDict α β) : Array (α × β) :=
-  self.entries.filterMap (·.toOption)
-
-@[inline] protected def beq
-  [BEq (α × β)] (self other : HashDict α β)
-: Bool := self.items == other.items
-
-instance [BEq (α × β)] : BEq (HashDict α β) := ⟨HashDict.beq⟩
-
-@[inline] def isEmpty (self : HashDict α β) : Bool :=
-  self.size == 0
-
-def keys (self : HashDict α β) : Array α :=
-  self.entries.filterMap (·.key?)
-
-def values (self : HashDict α β) : Array β :=
-  self.entries.filterMap (·.value?)
-
-@[inline] def getEntryIdx [Hashable α] [BEq α] (k : α) (self : HashDict α β) : Nat :=
-  self.raw.getEntryIdx k
-
 @[inline] def getEntryIdx?
-  [Hashable α] [BEq α] (k : α) (self : HashDict α β)
+  [Hashable α] [BEq α] (k : α) (self : TDict α β)
 : Option (Fin self.entries.size) :=
   let i := self.getEntryIdx k
   if h : i < self.entries.size then some ⟨i, h⟩ else none
 
 @[inline] def getEntry
-  [Hashable α] [BEq α] (k : α) (self : HashDict α β)
+  [Hashable α] [BEq α] (k : α) (self : TDict α β)
 : Entry α β :=
   let i := self.getEntryIdx k
   if h : i < self.entries.size then self.entries[i] else .none
 
-@[inline] def contains [Hashable α] [BEq α] (k : α) (self : HashDict α β) : Bool :=
-  self.raw.contains k
-
-structure Mem [Hashable α] [BEq α] (self : HashDict α β) (k : α)  where
+structure Mem [Hashable α] [BEq α] (self : TDict α β) (k : α)  where
   getEntryIdx_lt : self.getEntryIdx k < self.entries.size
   isSome_getElem_entries : self.entries[self.getEntryIdx k].isSome
 
-instance [Hashable α] [BEq α] : Membership α (HashDict α β) :=
+instance [Hashable α] [BEq α] : Membership α (TDict α β) :=
   ⟨fun d a => contains a d⟩
 
 @[simp] theorem contains_iff_mem
-  [Hashable α] [BEq α] {self : HashDict α β} :
+  [Hashable α] [BEq α] {self : TDict α β} :
   contains k self ↔ k ∈ self
 := Iff.intro id id
 
 theorem mem_iff_mem
-  [Hashable α] [BEq α] {self : HashDict α β} :
+  [Hashable α] [BEq α] {self : TDict α β} :
   k ∈ self ↔ self.Mem k
 := by
-  simp only [← contains_iff_mem, contains, Raw.contains]
+  simp only [← contains_iff_mem, contains, TDict.contains]
   apply Iff.intro
   · intro h
     split at h
     · next h_lt => exact ⟨h_lt, h⟩
     · simp at h
-  · intro h
-    have ⟨h_lt, h_isSome⟩ := h
-    simp only [getEntryIdx, entries] at h_lt h_isSome
+  · intro ⟨h_lt, h_isSome⟩
     simp [h_lt, h_isSome]
 
 theorem getEntryIdx_lt_of_mem
-  [Hashable α] [BEq α] {self : HashDict α β}
+  [Hashable α] [BEq α] {self : TDict α β}
   (h : k ∈ self) : self.getEntryIdx k < self.entries.size
 := Mem.getEntryIdx_lt (mem_iff_mem.mp h)
 
@@ -365,34 +341,14 @@ macro_rules
   `(tactic|with_reducible apply getEntryIdx_lt_of_mem; get_elem_tactic_extensible; done)
 
 theorem isSome_getElem_entries_of_mem
-  [Hashable α] [BEq α] {self : HashDict α β}
+  [Hashable α] [BEq α] {self : TDict α β}
   (h : k ∈ self) : self.entries[self.getEntryIdx k].isSome
 := Mem.isSome_getElem_entries (mem_iff_mem.mp h)
 
 @[inline] def get
-  [Hashable α] [BEq α] (k : α) (self : HashDict α β) (h : k ∈ self)
+  [Hashable α] [BEq α] (k : α) (self : TDict α β) (h : k ∈ self)
 : β := self.entries[self.getEntryIdx k].value (isSome_getElem_entries_of_mem h)
 
-@[inline] def get?
-  [Hashable α] [BEq α] (k : α) (self : HashDict α β)
-: Option β := self.getEntry k |>.value?
-
-instance [Hashable α] [BEq α] : GetElem? (HashDict α β) α β (fun d k => k ∈ d) where
+instance [Hashable α] [BEq α] : GetElem? (TDict α β) α β (fun d k => k ∈ d) where
   getElem d k h := get k d h
   getElem? d k := get? k d
-
-@[inline] def insert
-  [Hashable α] [BEq α] (self : HashDict α β) (k : α) (v : β)
-: HashDict α β := ⟨self.raw.insert k v⟩
-
-@[specialize] def ofArray [Hashable α] [BEq α] (items : Array (α × β)) : HashDict α β :=
-  items.foldl (init := emptyWithCapacity items.size) fun d (k, v) =>
-    d.insert k v
-
-@[inline] def erase
-  [Hashable α] [BEq α] (k : α) (self : HashDict α β)
-: HashDict α β := ⟨self.raw.erase k⟩
-
-/-- Remove erased entries from the dictionary. -/
-@[inline] def compress (self : HashDict α β) : HashDict α β :=
-  ⟨self.raw.compress⟩
